Reachability_Analysis/Reachability_Certificate.thy
@@ -1,6 +1,7 @@
 theory Reachability_Certificate
   imports Reachability_Analysis Grounded_PDDL.Grounded_PDDL
     Datalog_Certification.Datalog_Certificate
+    Tree_Decomp_Grounding_Common.Numeric_Free
 begin
 
 text \<open>\<^theory>\<open>Stratified_Datalog.Datalog\<close>'s \<^typ>\<open>('x, 'c) id\<close> constructors would otherwise capture
@@ -61,10 +62,10 @@ next
   show ?case
   proof (cases "p' = p")
     case True
-    then show ?thesis using g ih by (auto simp: Let_def)
+    thus ?thesis using g ih by (auto simp: Let_def)
   next
     case False
-    then show ?thesis using g ih by (simp add: Let_def)
+    thus ?thesis using g ih by (simp add: Let_def)
   qed
 qed
 
@@ -139,7 +140,7 @@ proof -
   proof
     fix a assume "a \<in> set args"
     then obtain i where "i < length args" "args ! i = a" by (auto simp: in_set_conv_nth)
-    then have "is_obj_of_type a (map snd (parameters h) ! i)"
+    hence "is_obj_of_type a (map snd (parameters h) ! i)"
       using assms unfolding action_params_match_def by (auto simp: list_all2_conv_all_nth)
     thus "a \<in> set const_names" using is_obj_of_type_const_name by blast
   qed
@@ -213,7 +214,7 @@ proof -
   have pos: "is_pos_conj pre"
   proof -
     have "\<forall>a\<in>set (actions D). is_pos_conj (ac_pre a)"
-      using relaxed_prob unfolding relaxed_prob_def by simp
+      using relaxed_prob by (auto simp: relaxed_prob_def relaxed_dom_def)
     hence "is_pos_conj (ac_pre ac)" using assms(2) by simp
     thus ?thesis using ac_eq by simp
   qed
@@ -295,17 +296,24 @@ fun dl_cond_rh :: "term atom formula \<Rightarrow> (predicate, variable, object)
 | "dl_cond_rh (\<^bold>\<not> (Atom (predAtm _ _))) = Some None"
 | "dl_cond_rh _ = None"
 
+text \<open>The shared datalog clause body of an action clause: one \<^const>\<open>PosLit\<close> per positive
+  precondition atom plus the surviving \<^const>\<open>Eql\<close>/\<^const>\<open>Neql\<close> equality guards. Every clause
+  emitted for the action clause (one per add-effect) carries this same body, so it is factored out.\<close>
+definition dl_clause_body :: "action_clause \<Rightarrow> (predicate, variable, object) rh list" where
+  "dl_clause_body cl =
+     map the (map dl_pos_rh (cl_pred_pre cl))
+     @ List.map_filter id (map the (map dl_cond_rh (cl_cond_pre cl)))"
+
 definition dl_clauses_of_action_clause :: "action_clause \<Rightarrow> pddl_dl_clause list" where
   [code]: "dl_clauses_of_action_clause cl \<equiv>
      (let conds = map dl_cond_rh (cl_cond_pre cl);
           pres = map dl_pos_rh (cl_pred_pre cl)
       in if None \<in> set conds \<or> None \<in> set pres then []
          else
-           let body = map the pres @ List.map_filter id (map the conds)
-           in List.map_filter
-                (\<lambda>f. case f of Atom (predAtm p ts) \<Rightarrow> Some (Cls p (map dl_id_of_term ts) body)
-                             | _ \<Rightarrow> None)
-                (cl_pos cl))"
+           List.map_filter
+             (\<lambda>f. case f of Atom (predAtm p ts) \<Rightarrow> Some (Cls p (map dl_id_of_term ts) (dl_clause_body cl))
+                          | _ \<Rightarrow> None)
+             (cl_pos cl))"
 
 fun dl_fact_clause :: "object atom formula \<Rightarrow> pddl_dl_clause option" where
   "dl_fact_clause (Atom (predAtm p args)) = Some (Cls p (map id.Cst args) [])"
@@ -352,17 +360,94 @@ text \<open>What the (relaxed, normalized) problem must guarantee for the generi
   \<^item> the initial facts are predicate atoms (their fact clauses survive the translation);
   \<^item> the object universe is non-empty (parameters that do not occur in a clause still need a
     witness argument on the PDDL side).\<close>
+text \<open>Named per-action-clause sub-conditions of the bundle, so the definition and its rules read
+  declaratively instead of as a nested \<open>\<forall>\<close>/\<open>\<forall>x\<in>set\<close> term.\<close>
+definition dl_pre_translates :: "action_clause \<Rightarrow> bool" where
+  "dl_pre_translates cl \<longleftrightarrow> (\<forall>a \<in> set (cl_pred_pre cl). dl_pos_rh a \<noteq> None)"
+
+definition dl_adds_predAtoms :: "action_clause \<Rightarrow> bool" where
+  "dl_adds_predAtoms cl \<longleftrightarrow> (\<forall>a \<in> set (cl_pos cl). is_predAtom a)"
+
+definition dl_cond_translates :: "action_clause \<Rightarrow> bool" where
+  "dl_cond_translates cl \<longleftrightarrow> (\<forall>cnd \<in> set (cl_cond_pre cl).
+       dl_cond_rh cnd \<noteq> None \<or> (\<forall>args. \<not> satisfies_cond (cl_params cl) args cnd))"
+
+definition dl_clause_vars_params :: "action_clause \<Rightarrow> bool" where
+  "dl_clause_vars_params cl \<longleftrightarrow> (\<forall>dcl \<in> set (dl_clauses_of_action_clause cl).
+       set (cls_vars dcl) \<subseteq> set (map fst (cl_params cl)))"
+
 definition dl_bridge_wf where
-  "dl_bridge_wf R \<equiv>
+  "dl_bridge_wf R \<longleftrightarrow>
      (\<forall>cl \<in> set (ast_classical_problem.a_clauses R).
-        (\<forall>a \<in> set (cl_pred_pre cl). dl_pos_rh a \<noteq> None)
-        \<and> (\<forall>a \<in> set (cl_pos cl). is_predAtom a)
-        \<and> (\<forall>cnd \<in> set (cl_cond_pre cl).
-             dl_cond_rh cnd \<noteq> None \<or> (\<forall>args. \<not> satisfies_cond (cl_params cl) args cnd))
-        \<and> (\<forall>dcl \<in> set (dl_clauses_of_action_clause cl).
-             set (cls_vars dcl) \<subseteq> set (map fst (cl_params cl))))
+        dl_pre_translates cl \<and> dl_adds_predAtoms cl
+        \<and> dl_cond_translates cl \<and> dl_clause_vars_params cl)
      \<and> (\<forall>f \<in> set (ast_classical_problem.init' R). is_predAtom f)
      \<and> ast_classical_problem.const_names R \<noteq> []"
+
+text \<open>Introduction / elimination / destruction rules for the bundle. Following the project
+  convention, they are stated with the \<open>\<And>\<close> (big-and) meta-binder rather than HOL \<open>\<forall>\<close>/\<open>\<forall>x\<in>set\<close>,
+  and reach all the way down to the element-level facts, so consuming proofs never re-derive the
+  nested quantifier structure.\<close>
+lemma dl_bridge_wfI [intro]:
+  assumes "\<And>cl a. cl \<in> set (ast_classical_problem.a_clauses R) \<Longrightarrow> a \<in> set (cl_pred_pre cl)
+             \<Longrightarrow> dl_pos_rh a \<noteq> None"
+    and "\<And>cl a. cl \<in> set (ast_classical_problem.a_clauses R) \<Longrightarrow> a \<in> set (cl_pos cl)
+             \<Longrightarrow> is_predAtom a"
+    and "\<And>cl cnd. cl \<in> set (ast_classical_problem.a_clauses R) \<Longrightarrow> cnd \<in> set (cl_cond_pre cl)
+             \<Longrightarrow> dl_cond_rh cnd \<noteq> None \<or> (\<forall>args. \<not> satisfies_cond (cl_params cl) args cnd)"
+    and "\<And>cl dcl. cl \<in> set (ast_classical_problem.a_clauses R)
+             \<Longrightarrow> dcl \<in> set (dl_clauses_of_action_clause cl)
+             \<Longrightarrow> set (cls_vars dcl) \<subseteq> set (map fst (cl_params cl))"
+    and "\<And>f. f \<in> set (ast_classical_problem.init' R) \<Longrightarrow> is_predAtom f"
+    and "ast_classical_problem.const_names R \<noteq> []"
+  shows "dl_bridge_wf R"
+  using assms unfolding dl_bridge_wf_def dl_pre_translates_def dl_adds_predAtoms_def
+    dl_cond_translates_def dl_clause_vars_params_def by blast
+
+lemma dl_bridge_wfE [elim]:
+  assumes "dl_bridge_wf R"
+  obtains "\<And>cl a. cl \<in> set (ast_classical_problem.a_clauses R) \<Longrightarrow> a \<in> set (cl_pred_pre cl)
+             \<Longrightarrow> dl_pos_rh a \<noteq> None"
+    and "\<And>cl a. cl \<in> set (ast_classical_problem.a_clauses R) \<Longrightarrow> a \<in> set (cl_pos cl)
+             \<Longrightarrow> is_predAtom a"
+    and "\<And>cl cnd. cl \<in> set (ast_classical_problem.a_clauses R) \<Longrightarrow> cnd \<in> set (cl_cond_pre cl)
+             \<Longrightarrow> dl_cond_rh cnd \<noteq> None \<or> (\<forall>args. \<not> satisfies_cond (cl_params cl) args cnd)"
+    and "\<And>cl dcl. cl \<in> set (ast_classical_problem.a_clauses R)
+             \<Longrightarrow> dcl \<in> set (dl_clauses_of_action_clause cl)
+             \<Longrightarrow> set (cls_vars dcl) \<subseteq> set (map fst (cl_params cl))"
+    and "\<And>f. f \<in> set (ast_classical_problem.init' R) \<Longrightarrow> is_predAtom f"
+    and "ast_classical_problem.const_names R \<noteq> []"
+  using assms unfolding dl_bridge_wf_def dl_pre_translates_def dl_adds_predAtoms_def
+    dl_cond_translates_def dl_clause_vars_params_def by blast
+
+lemma dl_bridge_wf_pred_preD [dest]:
+  "dl_bridge_wf R \<Longrightarrow> cl \<in> set (ast_classical_problem.a_clauses R) \<Longrightarrow> a \<in> set (cl_pred_pre cl)
+     \<Longrightarrow> dl_pos_rh a \<noteq> None"
+  unfolding dl_bridge_wf_def dl_pre_translates_def by blast
+
+lemma dl_bridge_wf_posD [dest]:
+  "dl_bridge_wf R \<Longrightarrow> cl \<in> set (ast_classical_problem.a_clauses R) \<Longrightarrow> a \<in> set (cl_pos cl)
+     \<Longrightarrow> is_predAtom a"
+  unfolding dl_bridge_wf_def dl_adds_predAtoms_def by blast
+
+lemma dl_bridge_wf_condD [dest]:
+  "dl_bridge_wf R \<Longrightarrow> cl \<in> set (ast_classical_problem.a_clauses R) \<Longrightarrow> cnd \<in> set (cl_cond_pre cl)
+     \<Longrightarrow> dl_cond_rh cnd \<noteq> None \<or> (\<forall>args. \<not> satisfies_cond (cl_params cl) args cnd)"
+  unfolding dl_bridge_wf_def dl_cond_translates_def by blast
+
+lemma dl_bridge_wf_varsD [dest]:
+  "dl_bridge_wf R \<Longrightarrow> cl \<in> set (ast_classical_problem.a_clauses R)
+     \<Longrightarrow> dcl \<in> set (dl_clauses_of_action_clause cl)
+     \<Longrightarrow> set (cls_vars dcl) \<subseteq> set (map fst (cl_params cl))"
+  unfolding dl_bridge_wf_def dl_clause_vars_params_def by blast
+
+lemma dl_bridge_wf_initD [dest]:
+  "dl_bridge_wf R \<Longrightarrow> f \<in> set (ast_classical_problem.init' R) \<Longrightarrow> is_predAtom f"
+  unfolding dl_bridge_wf_def by blast
+
+lemma dl_bridge_wf_const_namesD [dest]:
+  "dl_bridge_wf R \<Longrightarrow> ast_classical_problem.const_names R \<noteq> []"
+  unfolding dl_bridge_wf_def by blast
 
 
 section \<open>PDDL reachability is the minimal model of the translated program\<close>
@@ -395,13 +480,19 @@ text \<open>The semantic relation between an accepted certificate and PDDL reach
 context pddl_datalog
 begin
 
+text \<open>The translated program \<^const>\<open>dl_rules\<close> of this (relaxed, normalized) problem, over the
+  object universe \<^const>\<open>const_names\<close>, as an interpretation of the assumption-free
+  \<^locale>\<open>datalog_prog\<close>. Its inductive least model is available as \<open>dl_prog.derivable\<close>
+  (= \<^term>\<open>datalog_prog.derivable (set const_names) (set (dl_rules P))\<close>).\<close>
+sublocale dl_prog: datalog_prog "set const_names" "set (dl_rules P)" .
+
 text \<open>\<^bold>\<open>Base core (still \<^bold>\<open>sorry\<close>):\<close> every initial fact is derivable --- it is the head of a
   bodyless ground fact clause \<^const>\<open>dl_fact_clause\<close> in \<^const>\<open>dl_rules\<close>, fired by the vacuous
   substitution.\<close>
 lemma derivable_init:
   assumes wf: "dl_bridge_wf P"
     and mem: "Atom (predAtm p xs) \<in> fst I"
-  shows "datalog_prog.derivable (set const_names) (set (dl_rules P)) (p, xs)"
+  shows "dl_prog.derivable (p, xs)"
 proof -
   from mem have "Atom (predAtm p xs) \<in> set (init P)"
     unfolding I_def by simp
@@ -416,11 +507,11 @@ proof -
   have g: "\<forall>gd\<in>set (cls_guards (Cls p (map id.Cst xs) [] :: pddl_dl_clause)).
              eval_guard (\<lambda>_. undefined) gd" by (simp add: cls_guards_def)
   have b: "\<forall>a\<in>set (cls_body_atoms (Cls p (map id.Cst xs) [] :: pddl_dl_clause)).
-             datalog_prog.derivable (set const_names) (set (dl_rules P)) (subst_atom (\<lambda>_. undefined) a)"
+             dl_prog.derivable (subst_atom (\<lambda>_. undefined) a)"
     by (simp add: cls_body_atoms_def List.map_filter_simps)
-  have "datalog_prog.derivable (set const_names) (set (dl_rules P))
+  have "dl_prog.derivable
           (subst_atom (\<lambda>_. undefined) (the_lh (Cls p (map id.Cst xs) [] :: pddl_dl_clause)))"
-    using datalog_prog.derivable.derive[OF cl v g b] .
+    using dl_prog.derivable.derive[OF cl v g b] .
   thus ?thesis by (simp add: subst_atom_def comp_def)
 qed
 
@@ -439,7 +530,7 @@ lemma ac_arg_in_const_names:
 proof -
   from assms(2) obtain i where "i < length args" "args ! i = a"
     by (auto simp: in_set_conv_nth)
-  then have "is_obj_of_type a (map snd (parameters h) ! i)"
+  hence "is_obj_of_type a (map snd (parameters h) ! i)"
     using assms(1) unfolding action_params_match_def by (auto simp: list_all2_conv_all_nth)
   thus ?thesis using is_obj_of_type_const_name by blast
 qed
@@ -471,17 +562,243 @@ lemma dl_cond_rh_eval_guard:
   by (cases cnd rule: dl_cond_rh.cases)
      (auto simp del: ac_tsubst_def simp add: valuation_def subst_id_dl_id_term)
 
-text \<open>\<^bold>\<open>Step core (still \<^bold>\<open>sorry\<close>):\<close> the add-effects of an enabled action are derivable, given
+text \<open>Shape of the translated literals: \<^const>\<open>dl_pos_rh\<close> yields either nothing or a positive
+  body literal; \<^const>\<open>dl_cond_rh\<close> yields nothing, the drop marker \<open>Some None\<close>, or an equality
+  guard. These pin down the body of a translated action clause.\<close>
+lemma dl_pos_rh_form: "dl_pos_rh a = None \<or> (\<exists>p ids. dl_pos_rh a = Some (PosLit p ids))"
+  by (cases a rule: dl_pos_rh.cases) auto
+
+lemma dl_pos_rh_Some:
+  assumes "dl_pos_rh a = Some r"
+  shows "\<exists>p ts. a = Atom (predAtm p ts) \<and> r = PosLit p (map dl_id_of_term ts)"
+  using assms by (cases a rule: dl_pos_rh.cases) auto
+
+lemma dl_cond_rh_form:
+  "dl_cond_rh c = None \<or> dl_cond_rh c = Some None
+   \<or> (\<exists>g. dl_cond_rh c = Some (Some g) \<and> is_dl_guard g)"
+  by (cases c rule: dl_cond_rh.cases) auto
+
+text \<open>When no precondition/condition literal fails to translate, the clause produced for an
+  add-effect predicate atom of an action clause is in \<^const>\<open>dl_clauses_of_action_clause\<close>.\<close>
+lemma dl_clause_of_pos_mem:
+  assumes nc: "None \<notin> set (map dl_cond_rh (cl_cond_pre cl))"
+    and np: "None \<notin> set (map dl_pos_rh (cl_pred_pre cl))"
+    and mem: "Atom (predAtm p ts) \<in> set (cl_pos cl)"
+  shows "Cls p (map dl_id_of_term ts) (dl_clause_body cl) \<in> set (dl_clauses_of_action_clause cl)"
+  using assms
+  by (auto simp: dl_clauses_of_action_clause_def Let_def set_map_filter' image_iff
+           intro!: bexI[where x="Atom (predAtm p ts)"])
+
+text \<open>Every guard of a translated action clause comes from an equality condition literal.\<close>
+lemma guard_from_cond:
+  assumes nc: "None \<notin> set (map dl_cond_rh (cl_cond_pre cl))"
+    and np: "None \<notin> set (map dl_pos_rh (cl_pred_pre cl))"
+    and g: "gd \<in> set (cls_guards (Cls p ids (dl_clause_body cl)))"
+  shows "\<exists>cnd \<in> set (cl_cond_pre cl). dl_cond_rh cnd = Some (Some gd)"
+proof -
+  let ?A = "map the (map dl_pos_rh (cl_pred_pre cl))"
+  let ?Bc = "List.map_filter id (map the (map dl_cond_rh (cl_cond_pre cl)))"
+  from g have gdf: "gd \<in> set (filter is_dl_guard (?A @ ?Bc))"
+    by (simp add: cls_guards_def dl_clause_body_def)
+  hence guard: "is_dl_guard gd" and inAB: "gd \<in> set ?A \<or> gd \<in> set ?Bc" by auto
+  have notA: "gd \<notin> set ?A"
+  proof
+    assume "gd \<in> set ?A"
+    then obtain a where a: "a \<in> set (cl_pred_pre cl)" and gd_eq: "gd = the (dl_pos_rh a)" by auto
+    from a have m: "dl_pos_rh a \<in> set (map dl_pos_rh (cl_pred_pre cl))" by auto
+    have nn: "dl_pos_rh a \<noteq> None"
+    proof
+      assume "dl_pos_rh a = None"
+      hence "None \<in> set (map dl_pos_rh (cl_pred_pre cl))" using m by simp
+      thus False using np by simp
+    qed
+    with dl_pos_rh_form[of a] obtain p' ids' where "dl_pos_rh a = Some (PosLit p' ids')" by auto
+    thus False using gd_eq guard by simp
+  qed
+  hence "gd \<in> set ?Bc" using inAB by simp
+  hence "Some gd \<in> set (map the (map dl_cond_rh (cl_cond_pre cl)))"
+    by (auto simp: set_map_filter')
+  then obtain cnd where cnd: "cnd \<in> set (cl_cond_pre cl)" and someq: "the (dl_cond_rh cnd) = Some gd" by auto
+  from cnd have m2: "dl_cond_rh cnd \<in> set (map dl_cond_rh (cl_cond_pre cl))" by auto
+  have nn2: "dl_cond_rh cnd \<noteq> None"
+  proof
+    assume "dl_cond_rh cnd = None"
+    hence "None \<in> set (map dl_cond_rh (cl_cond_pre cl))" using m2 by simp
+    thus False using nc by simp
+  qed
+  hence "dl_cond_rh cnd = Some (Some gd)" using someq by (cases "dl_cond_rh cnd") auto
+  thus ?thesis using cnd by blast
+qed
+
+text \<open>Every body atom of a translated action clause comes from a positive precondition atom.\<close>
+lemma body_atom_from_pre:
+  assumes nc: "None \<notin> set (map dl_cond_rh (cl_cond_pre cl))"
+    and np: "None \<notin> set (map dl_pos_rh (cl_pred_pre cl))"
+    and b: "ba \<in> set (cls_body_atoms (Cls p ids (dl_clause_body cl)))"
+  shows "\<exists>p' ts'. Atom (predAtm p' ts') \<in> set (cl_pred_pre cl) \<and> ba = (p', map dl_id_of_term ts')"
+proof -
+  let ?A = "map the (map dl_pos_rh (cl_pred_pre cl))"
+  let ?Bc = "List.map_filter id (map the (map dl_cond_rh (cl_cond_pre cl)))"
+  from b have "ba \<in> set (List.map_filter rh_body_atom (?A @ ?Bc))"
+    by (simp add: cls_body_atoms_def dl_clause_body_def)
+  then obtain x where x: "x \<in> set (?A @ ?Bc)" and rb: "rh_body_atom x = Some ba"
+    by (auto simp: set_map_filter')
+  have "x \<notin> set ?Bc"
+  proof
+    assume "x \<in> set ?Bc"
+    hence "Some x \<in> set (map the (map dl_cond_rh (cl_cond_pre cl)))"
+      by (auto simp: set_map_filter')
+    then obtain cnd where cnd: "cnd \<in> set (cl_cond_pre cl)" and sx: "the (dl_cond_rh cnd) = Some x" by auto
+    from cnd have m2: "dl_cond_rh cnd \<in> set (map dl_cond_rh (cl_cond_pre cl))" by auto
+    have "dl_cond_rh cnd \<noteq> None"
+    proof
+      assume "dl_cond_rh cnd = None"
+      hence "None \<in> set (map dl_cond_rh (cl_cond_pre cl))" using m2 by simp
+      thus False using nc by simp
+    qed
+    hence "is_dl_guard x" using dl_cond_rh_form[of cnd] sx by auto
+    thus False using rb by (cases x) auto
+  qed
+  hence "x \<in> set ?A" using x by simp
+  then obtain a where a: "a \<in> set (cl_pred_pre cl)" and xeq: "x = the (dl_pos_rh a)" by auto
+  from a have m: "dl_pos_rh a \<in> set (map dl_pos_rh (cl_pred_pre cl))" by auto
+  have "dl_pos_rh a \<noteq> None"
+  proof
+    assume "dl_pos_rh a = None"
+    hence "None \<in> set (map dl_pos_rh (cl_pred_pre cl))" using m by simp
+    thus False using np by simp
+  qed
+  then obtain r where r: "dl_pos_rh a = Some r" by auto
+  with dl_pos_rh_Some obtain p' ts' where aeq: "a = Atom (predAtm p' ts')"
+    and req: "r = PosLit p' (map dl_id_of_term ts')" by blast
+  from xeq r req have "x = PosLit p' (map dl_id_of_term ts')" by simp
+  hence "ba = (p', map dl_id_of_term ts')" using rb by simp
+  thus ?thesis using aeq a by auto
+qed
+
+text \<open>\<^bold>\<open>Step core:\<close> the add-effects of an enabled action are derivable, given
   that the current world-model facts are. The fired action's translated clause supplies the
   generic ground instance (substitution from the action arguments, body atoms from the
   hypothesis, equality guards from \<^const>\<open>satisfies_conds\<close>).\<close>
 lemma derivable_step_adds:
   assumes wf: "dl_bridge_wf P" and en: "plan_action_enabled a M"
     and IH: "\<forall>p xs. Atom (predAtm p xs) \<in> fst M
-               \<longrightarrow> datalog_prog.derivable (set const_names) (set (dl_rules P)) (p, xs)"
+               \<longrightarrow> dl_prog.derivable (p, xs)"
     and mem: "Atom (predAtm p xs) \<in> set (adds (effect ((the \<circ> res_inst) a)))"
-  shows "datalog_prog.derivable (set const_names) (set (dl_rules P)) (p, xs)"
-  sorry
+  shows "dl_prog.derivable (p, xs)"
+proof -
+  obtain n args where a_eq: "a = SimplePlanAction n args" by (cases a)
+  from en have wfa: "wf_classical_plan_action (SimplePlanAction n args)"
+    unfolding a_eq plan_action_enabled_def by simp
+  from wfa obtain sch where res: "resolve_classical_action_schema n = Some sch"
+    by (auto simp: wf_classical_plan_action_simple split: option.splits)
+  obtain n' ps pre ad dl nl where sch_eq:
+      "sch = SimpleActionSchema (ActionHead n' ps) (SimpleActionBody pre (Effect ad dl nl))"
+    by (metis ast_classical_action_schema_cases_unfold ast_effect.exhaust)
+  from wfa res have pm0: "action_params_match (ActionHead n' ps) args"
+    by (simp add: wf_classical_plan_action_simple sch_eq)
+  from res have sch_mem: "sch \<in> set (actions D)" and sch_name: "ac_name sch = n"
+    unfolding resolve_classical_action_schema_def by (auto dest: index_by_eq_SomeD)
+  from sch_name sch_eq have n'_n: "n' = n" by simp
+  have sch_eq': "sch = SimpleActionSchema (ActionHead n ps) (SimpleActionBody pre (Effect ad dl nl))"
+    using sch_eq n'_n by simp
+  have pm: "action_params_match (ActionHead n ps) args" using pm0 n'_n by simp
+  define cl_ac where "cl_ac = as_action_clause sch"
+  have clparams: "cl_params cl_ac = ps" and clpred: "cl_pred_pre cl_ac = pos_lits_of pre"
+    and clcond: "cl_cond_pre cl_ac = cond_lits_of pre" and clpos: "cl_pos cl_ac = ad"
+    unfolding cl_ac_def sch_eq' by simp_all
+  have cl_ac_mem: "cl_ac \<in> set a_clauses"
+    unfolding cl_ac_def a_clauses_def using sch_mem by simp
+  have np: "None \<notin> set (map dl_pos_rh (cl_pred_pre cl_ac))"
+    using dl_bridge_wf_pred_preD[OF wf cl_ac_mem] by fastforce
+  have posprop: "\<forall>a \<in> set (cl_pos cl_ac). is_predAtom a"
+    using dl_bridge_wf_posD[OF wf cl_ac_mem] by blast
+  have condwf: "\<forall>cnd \<in> set (cl_cond_pre cl_ac).
+       dl_cond_rh cnd \<noteq> None \<or> (\<forall>args. \<not> satisfies_cond ps args cnd)"
+    unfolding clparams[symmetric] using dl_bridge_wf_condD[OF wf cl_ac_mem] by blast
+  have varsub: "\<forall>dcl \<in> set (dl_clauses_of_action_clause cl_ac). set (cls_vars dcl) \<subseteq> set (map fst ps)"
+    unfolding clparams[symmetric] using dl_bridge_wf_varsD[OF wf cl_ac_mem] by blast
+  have en': "plan_action_enabled (SimplePlanAction n args) M" using en a_eq by simp
+  note ecb = enabled_clause_body[OF en' sch_mem sch_name]
+  have pos_part: "set (map (map_atom_fmla (ac_tsubst ps args)) (cl_pred_pre cl_ac)) \<subseteq> fst M"
+    using ecb by (simp add: cl_ac_def[symmetric] clparams)
+  have sat: "satisfies_conds ps (cl_cond_pre cl_ac) args"
+    using ecb by (simp add: cl_ac_def[symmetric] clparams)
+  have nc: "None \<notin> set (map dl_cond_rh (cl_cond_pre cl_ac))"
+  proof -
+    have "\<forall>cnd \<in> set (cl_cond_pre cl_ac). dl_cond_rh cnd \<noteq> None"
+    proof
+      fix cnd assume c: "cnd \<in> set (cl_cond_pre cl_ac)"
+      from sat c have "satisfies_cond ps args cnd" by (simp add: list_all_iff)
+      moreover from condwf c have "dl_cond_rh cnd \<noteq> None \<or> (\<forall>args'. \<not> satisfies_cond ps args' cnd)" by blast
+      ultimately show "dl_cond_rh cnd \<noteq> None" by blast
+    qed
+    thus ?thesis by auto
+  qed
+  have adds_eq: "adds (effect ((the \<circ> res_inst) a)) = consequence_of cl_ac args"
+    using res_inst_adds_eq_consequence[OF sch_mem[unfolded sch_eq']]
+    unfolding a_eq cl_ac_def sch_eq' by (simp add: comp_def)
+  have conseq: "consequence_of cl_ac args = map (map_atom_fmla (ac_tsubst ps args)) (cl_pos cl_ac)"
+    unfolding cl_ac_def sch_eq' by simp
+  from mem adds_eq conseq
+  have memc: "Atom (predAtm p xs) \<in> set (map (map_atom_fmla (ac_tsubst ps args)) (cl_pos cl_ac))" by simp
+  then obtain f0 where f0: "f0 \<in> set (cl_pos cl_ac)"
+    and f0eq: "Atom (predAtm p xs) = map_atom_fmla (ac_tsubst ps args) f0" by auto
+  from posprop f0 have "is_predAtom f0" by blast
+  then obtain p0 ts0 where f0_pred: "f0 = Atom (predAtm p0 ts0)"
+    by (cases f0 rule: is_predAtom.cases) auto
+  have pxs: "p = p0 \<and> xs = map (ac_tsubst ps args) ts0"
+    using f0eq f0_pred by simp
+  have mem0: "Atom (predAtm p0 ts0) \<in> set (cl_pos cl_ac)" using f0 f0_pred by simp
+  define sig where "sig = (\<lambda>v. ac_tsubst ps args (term.VAR v))"
+  define B where "B = dl_clause_body cl_ac"
+  have clmem: "Cls p0 (map dl_id_of_term ts0) B \<in> set (dl_clauses_of_action_clause cl_ac)"
+    unfolding B_def by (rule dl_clause_of_pos_mem[OF nc np mem0])
+  have clrules: "Cls p0 (map dl_id_of_term ts0) B \<in> set (dl_rules P)"
+    unfolding dl_rules_def using clmem cl_ac_mem by auto
+  have vars: "\<forall>x \<in> set (cls_vars (Cls p0 (map dl_id_of_term ts0) B)). sig x \<in> set const_names"
+  proof
+    fix x assume "x \<in> set (cls_vars (Cls p0 (map dl_id_of_term ts0) B))"
+    hence xp: "x \<in> set (map fst ps)" using varsub clmem by blast
+    have "sig x \<in> set args" unfolding sig_def using ac_tsubst_var_in_args[OF pm xp] .
+    thus "sig x \<in> set const_names" using ac_arg_in_const_names[OF pm] by blast
+  qed
+  have guards: "\<forall>g \<in> set (cls_guards (Cls p0 (map dl_id_of_term ts0) B)). eval_guard sig g"
+  proof
+    fix g assume "g \<in> set (cls_guards (Cls p0 (map dl_id_of_term ts0) B))"
+    hence ing: "g \<in> set (cls_guards (Cls p0 (map dl_id_of_term ts0) (dl_clause_body cl_ac)))"
+      unfolding B_def .
+    from guard_from_cond[OF nc np ing] obtain cnd where cnd: "cnd \<in> set (cl_cond_pre cl_ac)"
+      and dcr: "dl_cond_rh cnd = Some (Some g)" by blast
+    from sat cnd have "satisfies_cond ps args cnd" by (simp add: list_all_iff)
+    from dl_cond_rh_eval_guard[OF dcr this] show "eval_guard sig g" unfolding sig_def .
+  qed
+  have bodyder: "\<forall>a \<in> set (cls_body_atoms (Cls p0 (map dl_id_of_term ts0) B)).
+      dl_prog.derivable (subst_atom sig a)"
+  proof
+    fix a assume "a \<in> set (cls_body_atoms (Cls p0 (map dl_id_of_term ts0) B))"
+    hence ainb: "a \<in> set (cls_body_atoms (Cls p0 (map dl_id_of_term ts0) (dl_clause_body cl_ac)))"
+      unfolding B_def .
+    from body_atom_from_pre[OF nc np ainb] obtain p' ts'
+      where prem: "Atom (predAtm p' ts') \<in> set (cl_pred_pre cl_ac)"
+        and aeq: "a = (p', map dl_id_of_term ts')" by blast
+    have sa: "subst_atom sig a = (p', map (ac_tsubst ps args) ts')"
+      unfolding aeq subst_atom_def
+      by (simp add: sig_def subst_id_dl_id_term comp_def del: ac_tsubst_def)
+    have "map_atom_fmla (ac_tsubst ps args) (Atom (predAtm p' ts')) \<in> fst M"
+      using pos_part prem by auto
+    hence "Atom (predAtm p' (map (ac_tsubst ps args) ts')) \<in> fst M" by simp
+    hence "dl_prog.derivable (p', map (ac_tsubst ps args) ts')" using IH by blast
+    thus "dl_prog.derivable (subst_atom sig a)" unfolding sa .
+  qed
+  have der: "dl_prog.derivable
+        (subst_atom sig (the_lh (Cls p0 (map dl_id_of_term ts0) B)))"
+    by (rule dl_prog.derivable.derive[OF clrules vars guards bodyder])
+  have lh: "subst_atom sig (the_lh (Cls p0 (map dl_id_of_term ts0) B)) = (p, xs)"
+    unfolding subst_atom_def
+    by (simp add: sig_def subst_id_dl_id_term comp_def pxs del: ac_tsubst_def)
+  from der lh show ?thesis by simp
+qed
 
 text \<open>The derivability invariant carried along a valid plan, proved from \<open>derivable_step_adds\<close>:
   every fact of a reachable world model is derivable, given the initial facts are.\<close>
@@ -489,9 +806,9 @@ lemma derivable_invariant:
   assumes wf: "dl_bridge_wf P"
   shows "valid_classical_plan_alt M \<pi>s M'
          \<Longrightarrow> (\<forall>p xs. Atom (predAtm p xs) \<in> fst M
-                \<longrightarrow> datalog_prog.derivable (set const_names) (set (dl_rules P)) (p, xs))
+                \<longrightarrow> dl_prog.derivable (p, xs))
          \<Longrightarrow> (\<forall>p xs. Atom (predAtm p xs) \<in> fst M'
-                \<longrightarrow> datalog_prog.derivable (set const_names) (set (dl_rules P)) (p, xs))"
+                \<longrightarrow> dl_prog.derivable (p, xs))"
 proof (induction \<pi>s arbitrary: M)
   case Nil thus ?case by simp
 next
@@ -504,15 +821,15 @@ next
                  = (L - set (dels (effect ?a'))) \<union> set (adds (effect ?a'))"
     unfolding execute_plan_action_def M using apply_ground_action_alt[of ?a' L N] by simp
   have step: "\<forall>p xs. Atom (predAtm p xs) \<in> fst (execute_plan_action a M)
-                \<longrightarrow> datalog_prog.derivable (set const_names) (set (dl_rules P)) (p, xs)"
+                \<longrightarrow> dl_prog.derivable (p, xs)"
   proof (intro allI impI)
     fix p xs assume "Atom (predAtm p xs) \<in> fst (execute_plan_action a M)"
-    then have "Atom (predAtm p xs) \<in> L \<or> Atom (predAtm p xs) \<in> set (adds (effect ?a'))"
+    hence "Atom (predAtm p xs) \<in> L \<or> Atom (predAtm p xs) \<in> set (adds (effect ?a'))"
       unfolding fstM' by auto
-    thus "datalog_prog.derivable (set const_names) (set (dl_rules P)) (p, xs)"
+    thus "dl_prog.derivable (p, xs)"
     proof
       assume "Atom (predAtm p xs) \<in> L"
-      then have "Atom (predAtm p xs) \<in> fst M" using M by simp
+      hence "Atom (predAtm p xs) \<in> fst M" using M by simp
       thus ?thesis using Cons.prems(2) by blast
     next
       assume "Atom (predAtm p xs) \<in> set (adds (effect ?a'))"
@@ -526,44 +843,811 @@ subsection \<open>The minimal-model relation\<close>
 
 lemma achievable_imp_dl_derivable:
   assumes wf: "dl_bridge_wf P" and ach: "achievable f"
-  shows "datalog_prog.derivable (set const_names) (set (dl_rules P)) f"
+  shows "dl_prog.derivable f"
 proof -
   from ach obtain \<pi>s M where vp: "valid_classical_plan_alt I \<pi>s M"
     and mem: "Atom (uncurry predAtm f) \<in> fst M"
     unfolding achievable_def by auto
   obtain p xs where f: "f = (p, xs)" by (cases f)
   have init: "\<forall>p xs. Atom (predAtm p xs) \<in> fst I
-                \<longrightarrow> datalog_prog.derivable (set const_names) (set (dl_rules P)) (p, xs)"
+                \<longrightarrow> dl_prog.derivable (p, xs)"
     using derivable_init[OF wf] by blast
   have allM: "\<forall>p xs. Atom (predAtm p xs) \<in> fst M
-                \<longrightarrow> datalog_prog.derivable (set const_names) (set (dl_rules P)) (p, xs)"
+                \<longrightarrow> dl_prog.derivable (p, xs)"
     using derivable_invariant[OF wf vp init] .
   have "Atom (predAtm p xs) \<in> fst M" using mem f by simp
-  with allM have "datalog_prog.derivable (set const_names) (set (dl_rules P)) (p, xs)" by blast
+  hence "dl_prog.derivable (p, xs)" using allM by blast
   thus ?thesis using f by simp
 qed
 
-lemma dl_derivable_imp_achievable:
-  assumes wf: "dl_bridge_wf P"
-    and der: "datalog_prog.derivable (set const_names) (set (dl_rules P)) f"
-  shows "achievable f"
+subsection \<open>Delete-relaxation monotonicity infrastructure (for the tightness direction)\<close>
+
+text \<open>The reverse inclusion needs that the relaxed problem never deletes facts (delete
+  relaxation) and is numeric-free; neither is part of the abstract \<^locale>\<open>relaxed_problem\<close>, so
+  both are carried as explicit hypotheses (\<open>nd\<close> / \<open>nf\<close>). They hold for the pipeline's actual
+  relaxed, def-translated problem \<open>relax_prob (P\<^sub>T P)\<close>. Under them, facts only grow along a plan,
+  a plan replays from any larger start state, and an action clause whose body-atom instances are
+  achievable can be fired --- so every derivable fact is achievable.\<close>
+
+text \<open>One executed step only adds facts: under delete relaxation the resolved ground action has
+  no deletes, so the post-state facts are exactly the pre-state facts plus the action's adds.\<close>
+lemma execute_facts_eq:
+  assumes nd: "\<forall>a \<in> set (actions D). dels (ac_eff a) = []"
+    and en: "plan_action_enabled a M"
+  shows "fst (execute_plan_action a M) = fst M \<union> set (adds (effect ((the \<circ> res_inst) a)))"
 proof -
-  note ind = datalog_prog.derivable.induct[consumes 1, case_names step]
-  show ?thesis using der
-  proof (induction rule: ind)
-    case (step cl \<sigma>)
-    text \<open>\<^bold>\<open>(still \<^bold>\<open>sorry\<close>)\<close> \<open>cl\<close> is a clause of \<^const>\<open>dl_rules\<close>: either a translated
-      action clause --- fire that action, whose positive precondition body instances are
-      achievable by \<open>step.IH\<close> and whose equality guards hold --- or a bodyless fact clause from
-      \<open>init'\<close>, achievable at the initial model. Either way the head instance is achievable.\<close>
-    show ?case sorry
+  obtain n args where a_eq: "a = SimplePlanAction n args" by (cases a)
+  from en have wfa: "wf_classical_plan_action (SimplePlanAction n args)"
+    unfolding a_eq plan_action_enabled_def by (simp add: Let_def)
+  from wfa obtain sch where res: "resolve_classical_action_schema n = Some sch"
+    by (auto simp: wf_classical_plan_action_simple split: option.splits)
+  from res have sch_mem: "sch \<in> set (actions D)"
+    unfolding resolve_classical_action_schema_def by (auto dest: index_by_eq_SomeD)
+  have ri: "res_inst (SimplePlanAction n args)
+              = Some (instantiate_classical_action_schema sch args)"
+    using res by (simp add: res_inst_alt)
+  have eff: "effect ((the \<circ> res_inst) a)
+              = map_ast_effect (ac_tsubst (ac_params sch) args) (ac_eff sch)"
+    unfolding a_eq using ri by (simp add: instantiate_classical_action_schema_alt)
+  have "dels (ac_eff sch) = []" using nd sch_mem by blast
+  hence dels0: "dels (effect ((the \<circ> res_inst) a)) = []"
+    unfolding eff by (cases "ac_eff sch") simp
+  obtain L N where M: "M = (L, N)" by (cases M)
+  have "fst (execute_plan_action a M)
+          = (L - set (dels (effect ((the \<circ> res_inst) a)))) \<union> set (adds (effect ((the \<circ> res_inst) a)))"
+    unfolding execute_plan_action_def M by (simp add: apply_ground_action_alt)
+  thus ?thesis using dels0 M by auto
+qed
+
+lemma execute_grows:
+  assumes nd: "\<forall>a \<in> set (actions D). dels (ac_eff a) = []"
+    and en: "plan_action_enabled a M"
+  shows "fst M \<subseteq> fst (execute_plan_action a M)"
+  using execute_facts_eq[OF nd en] by blast
+
+text \<open>Hence facts persist along an entire valid plan.\<close>
+lemma plan_grows_facts:
+  assumes nd: "\<forall>a \<in> set (actions D). dels (ac_eff a) = []"
+    and "valid_classical_plan_alt M \<pi>s N"
+  shows "fst M \<subseteq> fst N"
+  using assms(2)
+proof (induction \<pi>s arbitrary: M)
+  case Nil thus ?case by simp
+next
+  case (Cons a \<pi>s)
+  from Cons.prems have en: "plan_action_enabled a M"
+    and rest: "valid_classical_plan_alt (execute_plan_action a M) \<pi>s N" by simp_all
+  have "fst M \<subseteq> fst (execute_plan_action a M)" by (rule execute_grows[OF nd en])
+  also have "\<dots> \<subseteq> fst N" using Cons.IH[OF rest] .
+  finally show ?case .
+qed
+
+text \<open>Reverse of \<open>un_and_map_semantics\<close>: a conjunction holds if all its \<open>un_and\<close> members do.\<close>
+lemma un_and_map_semantics_rev: "(\<forall>f \<in> set (un_and F). A \<Turnstile>\<^sub>m f) \<Longrightarrow> A \<Turnstile>\<^sub>m F"
+  by (induction F rule: un_and.induct) auto
+
+text \<open>A positive conjunction's truth under \<open>valuation\<close> is monotone in the fact set: its positive
+  predicate literals persist (membership grows), and its non-predicate (equality) literals are
+  model-independent.\<close>
+lemma valuation_pos_conj_mono:
+  assumes pc: "is_pos_conj F" and sub: "fst M1 \<subseteq> fst M2"
+    and v1: "valuation M1 \<Turnstile>\<^sub>m map_atom_fmla \<sigma> F"
+  shows "valuation M2 \<Turnstile>\<^sub>m map_atom_fmla \<sigma> F"
+proof (rule un_and_map_semantics_rev, unfold un_and_map_atom_fmla, rule ballI)
+  fix g assume "g \<in> set (map (map_atom_fmla \<sigma>) (un_and F))"
+  then obtain l where l: "l \<in> set (un_and F)" and g: "g = map_atom_fmla \<sigma> l" by auto
+  from l pc have posl: "is_pos_lit l" using is_pos_conj_alt by blast
+  from un_and_map_semantics[OF v1] l have v1l: "valuation M1 \<Turnstile>\<^sub>m map_atom_fmla \<sigma> l"
+    unfolding un_and_map_atom_fmla by auto
+  show "valuation M2 \<Turnstile>\<^sub>m g" unfolding g
+  proof (cases "is_predAtom l")
+    case True
+    then obtain p xs where l_eq: "l = Atom (predAtm p xs)"
+      by (cases l rule: is_predAtom.cases) auto
+    from v1l have "Atom (predAtm p (map \<sigma> xs)) \<in> fst M1"
+      unfolding l_eq by (simp add: valuation_def)
+    hence "Atom (predAtm p (map \<sigma> xs)) \<in> fst M2" using sub by blast
+    thus "valuation M2 \<Turnstile>\<^sub>m map_atom_fmla \<sigma> l" unfolding l_eq by (simp add: valuation_def)
+  next
+    case False
+    show "valuation M2 \<Turnstile>\<^sub>m map_atom_fmla \<sigma> l"
+      using cond_lit_model_indep[OF posl False] v1l by blast
   qed
 qed
 
+text \<open>An action enabled at \<open>M1\<close> is enabled at any fact-superset \<open>M2\<close>: relaxed (positive
+  conjunction) preconditions are monotone, and numeric-freeness makes the two numeric side
+  conditions vacuous (no numeric effects).\<close>
+lemma enabled_mono:
+  assumes nne: "\<forall>a \<in> set (actions D). numeric_effects (ac_eff a) = []"
+    and en: "plan_action_enabled a M1"
+    and sub: "fst M1 \<subseteq> fst M2"
+  shows "plan_action_enabled a M2"
+proof -
+  obtain n args where a_eq: "a = SimplePlanAction n args" by (cases a)
+  from en have wfa: "wf_classical_plan_action (SimplePlanAction n args)"
+    unfolding a_eq plan_action_enabled_def by (simp add: Let_def)
+  from en have val1: "valuation M1 \<Turnstile>\<^sub>m precondition ((the \<circ> res_inst) a)"
+    unfolding plan_action_enabled_def by (simp add: Let_def)
+  from wfa obtain sch where res: "resolve_classical_action_schema n = Some sch"
+    by (auto simp: wf_classical_plan_action_simple split: option.splits)
+  from res have sch_mem: "sch \<in> set (actions D)"
+    unfolding resolve_classical_action_schema_def by (auto dest: index_by_eq_SomeD)
+  have nm: "ac_name sch = n" using res res_aux sch_mem by blast
+  obtain n' ps pre ad dl nl where sch_eq0:
+      "sch = SimpleActionSchema (ActionHead n' ps) (SimpleActionBody pre (Effect ad dl nl))"
+    by (metis ast_classical_action_schema_cases_unfold ast_effect.exhaust)
+  have sch_eq: "sch = SimpleActionSchema (ActionHead n ps) (SimpleActionBody pre (Effect ad dl nl))"
+    using sch_eq0 nm by simp
+  have schmem': "SimpleActionSchema (ActionHead n ps) (SimpleActionBody pre (Effect ad dl nl)) \<in> set (actions D)"
+    using sch_mem sch_eq by simp
+  have ri: "res_inst (SimplePlanAction n args) = Some (GroundAction
+      (map_atom_fmla (ac_tsubst ps args) pre) (map_ast_effect (ac_tsubst ps args) (Effect ad dl nl)))"
+    by (rule res_inst_cond[OF schmem'])
+  have pre_eq: "precondition ((the \<circ> res_inst) a) = map_atom_fmla (ac_tsubst ps args) pre"
+    unfolding a_eq using ri by simp
+  have eff_eq: "effect ((the \<circ> res_inst) a) = map_ast_effect (ac_tsubst ps args) (Effect ad dl nl)"
+    unfolding a_eq using ri by simp
+  have ne0: "numeric_effects (ac_eff sch) = []" using nne sch_mem by blast
+  have nl0: "nl = []" using ne0 sch_eq by simp
+  have numeff0: "numeric_effects (effect ((the \<circ> res_inst) a)) = []"
+    unfolding eff_eq by (simp add: nl0)
+  have pos: "is_pos_conj pre"
+  proof -
+    have "\<forall>a\<in>set (actions D). is_pos_conj (ac_pre a)"
+      using relaxed_prob by (auto simp: relaxed_prob_def relaxed_dom_def)
+    hence "is_pos_conj (ac_pre sch)" using sch_mem by simp
+    thus ?thesis using sch_eq by simp
+  qed
+  show "plan_action_enabled a M2"
+    unfolding plan_action_enabled_def Let_def
+  proof (intro conjI)
+    show "wf_classical_plan_action a" using wfa unfolding a_eq .
+    show "numeric_effects_non_intrf ((the \<circ> res_inst) a)"
+      by (rule numeric_effects_non_intrf_no_numeric_effects[OF numeff0])
+    show "set (ast_effect_enumerate_rhs_primitive_numeric_expressions (effect ((the \<circ> res_inst) a)))
+            \<subseteq> dom (snd M2)"
+      using enumerate_rhs_pnes_no_numeric_effects[OF numeff0] by simp
+    show "valuation M2 \<Turnstile>\<^sub>m precondition ((the \<circ> res_inst) a)"
+      unfolding pre_eq by (rule valuation_pos_conj_mono[OF pos sub val1[unfolded pre_eq]])
+  qed
+qed
+
+text \<open>A valid plan replays from any fact-superset start state, reaching a fact-superset endpoint.\<close>
+lemma plan_replay_mono:
+  assumes nne: "\<forall>a \<in> set (actions D). numeric_effects (ac_eff a) = []"
+    and nd: "\<forall>a \<in> set (actions D). dels (ac_eff a) = []"
+    and "valid_classical_plan_alt M1 \<pi>s N1" and "fst M1 \<subseteq> fst M2"
+  shows "\<exists>N2. valid_classical_plan_alt M2 \<pi>s N2 \<and> fst N1 \<subseteq> fst N2"
+  using assms(3,4)
+proof (induction \<pi>s arbitrary: M1 M2)
+  case (Nil M1 M2)
+  hence "M1 = N1" by simp
+  thus ?case using Nil.prems(2) by auto
+next
+  case (Cons a \<pi>s M1 M2)
+  from Cons.prems(1) have en1: "plan_action_enabled a M1"
+    and rest1: "valid_classical_plan_alt (execute_plan_action a M1) \<pi>s N1" by simp_all
+  have en2: "plan_action_enabled a M2" by (rule enabled_mono[OF nne en1 Cons.prems(2)])
+  have step_sub: "fst (execute_plan_action a M1) \<subseteq> fst (execute_plan_action a M2)"
+    unfolding execute_facts_eq[OF nd en1] execute_facts_eq[OF nd en2]
+    using Cons.prems(2) by blast
+  from Cons.IH[OF rest1 step_sub] obtain N2
+    where v2: "valid_classical_plan_alt (execute_plan_action a M2) \<pi>s N2"
+      and sub2: "fst N1 \<subseteq> fst N2" by blast
+  have "valid_classical_plan_alt M2 (a # \<pi>s) N2" using en2 v2 by simp
+  thus ?case using sub2 by blast
+qed
+
+text \<open>A finite set of individually-achievable facts is jointly achievable: the per-fact plans
+  are concatenated, each replayed from the growing state, persistence keeping the earlier facts.\<close>
+lemma achievables_reach_common:
+  assumes nne: "\<forall>a \<in> set (actions D). numeric_effects (ac_eff a) = []"
+    and nd: "\<forall>a \<in> set (actions D). dels (ac_eff a) = []"
+    and "\<forall>f \<in> set fs. achievable f"
+  shows "\<exists>\<pi>s M. valid_classical_plan_alt I \<pi>s M \<and> (\<forall>f \<in> set fs. Atom (uncurry predAtm f) \<in> fst M)"
+  using assms(3)
+proof (induction fs)
+  case Nil
+  show ?case by (rule exI[of _ "[]"], rule exI[of _ I], simp)
+next
+  case (Cons f fs)
+  from Cons.prems have af: "achievable f" and rest: "\<forall>f \<in> set fs. achievable f" by simp_all
+  from Cons.IH[OF rest] obtain \<pi>s M
+    where vM: "valid_classical_plan_alt I \<pi>s M"
+      and fsM: "\<forall>g \<in> set fs. Atom (uncurry predAtm g) \<in> fst M" by blast
+  from af obtain \<rho>s Mf where vMf: "valid_classical_plan_alt I \<rho>s Mf"
+      and fMf: "Atom (uncurry predAtm f) \<in> fst Mf"
+    unfolding achievable_def by blast
+  have "fst I \<subseteq> fst M" by (rule plan_grows_facts[OF nd vM])
+  from plan_replay_mono[OF nne nd vMf this] obtain N
+    where vN: "valid_classical_plan_alt M \<rho>s N" and MfN: "fst Mf \<subseteq> fst N" by blast
+  have vIN: "valid_classical_plan_alt I (\<pi>s @ \<rho>s) N"
+    using valid_classical_plan_alt_append_intro[OF conjI[OF vM vN]] .
+  have fN: "Atom (uncurry predAtm f) \<in> fst N" using fMf MfN by blast
+  have "fst M \<subseteq> fst N" by (rule plan_grows_facts[OF nd vN])
+  hence "\<forall>g \<in> set (f # fs). Atom (uncurry predAtm g) \<in> fst N" using fsM fN by auto
+  thus ?case using vIN by blast
+qed
+
+text \<open>In a typeless (normalized) problem every object name has type \<open>\<omega>\<close>, so any object name
+  trivially matches the universal parameter type. This is the reverse of
+  \<open>is_obj_of_type_const_name\<close>, used to type the argument tuple reconstructed from a generic
+  substitution when firing a clause's action.\<close>
+lemma const_name_is_obj_of_type:
+  assumes "n \<in> set const_names"
+  shows "is_obj_of_type n \<omega>"
+proof -
+  have tless: "typeless_classical_problem"
+    using normalized_prob unfolding normalized_prob_def by simp
+  have all\<omega>: "T = \<omega>" if "(m, T) \<in> set all_consts" for m T
+  proof -
+    from that have "(m, T) \<in> set (consts D) \<or> (m, T) \<in> set (objects P)" by auto
+    thus ?thesis
+    proof
+      assume "(m, T) \<in> set (consts D)"
+      thus ?thesis using tless
+        unfolding typeless_classical_problem_def typeless_classical_domain_def
+          typeless_domain_signature_def by auto
+    next
+      assume "(m, T) \<in> set (objects P)"
+      thus ?thesis using tless unfolding typeless_classical_problem_def by auto
+    qed
+  qed
+  from assms have "n \<in> dom objT"
+    unfolding objT_alt by (simp add: dom_map_of_conv_image_fst)
+  then obtain oT where oT: "objT n = Some oT" by auto
+  hence "(n, oT) \<in> set all_consts" unfolding objT_alt by (auto dest: map_of_SomeD)
+  hence "oT = \<omega>" using all\<omega> by blast
+  thus ?thesis using oT unfolding is_obj_of_type_def by (simp add: of_type_refl)
+qed
+
+text \<open>An argument tuple of the right length drawn entirely from the object names matches an
+  action's (typeless) parameters. Used both to fire a fact clause's nullary-body action and to
+  type the tuple reconstructed from a generic substitution in the reverse-direction step case.\<close>
+lemma params_match_from_const_args:
+  assumes sch_mem: "sch \<in> set (actions D)"
+    and len: "length args = length (ac_params sch)"
+    and inc: "\<And>x. x \<in> set args \<Longrightarrow> x \<in> set const_names"
+  shows "action_params_match (ac_head sch) args"
+proof -
+  obtain n ps b where sch_eq: "sch = SimpleActionSchema (ActionHead n ps) b"
+    by (metis ast_classical_action_schema_cases_unfold)
+  have ph: "ac_head sch = ActionHead n ps" and pp: "ac_params sch = ps"
+    using sch_eq by simp_all
+  have types: "snd x = \<omega>" if "x \<in> set ps" for x
+    using param_types_omega[OF sch_mem] that pp by (cases x) auto
+  show ?thesis
+    unfolding ph action_params_match_def list_all2_conv_all_nth
+  proof (intro conjI allI impI)
+    show "length args = length (map snd (parameters (ActionHead n ps)))"
+      using len pp by simp
+  next
+    fix i assume i: "i < length args"
+    have "args ! i \<in> set const_names" using inc i by simp
+    hence "is_obj_of_type (args ! i) \<omega>" using const_name_is_obj_of_type by simp
+    moreover have "map snd (parameters (ActionHead n ps)) ! i = \<omega>"
+      using i len pp types by (simp add: nth_mem)
+    ultimately show "is_obj_of_type (args ! i) (map snd (parameters (ActionHead n ps)) ! i)"
+      by simp
+  qed
+qed
+
+text \<open>Inverting \<open>chosen_from\<close> on a uniform domain: a tuple chosen from \<open>n\<close> copies of \<open>S\<close> has
+  length \<open>n\<close> and lives in \<open>S\<close>.\<close>
+lemma chosen_from_replicate_dest:
+  "chosen_from (replicate n S) xs \<Longrightarrow> length xs = n \<and> (\<forall>x \<in> set xs. x \<in> set S)"
+proof (induction n arbitrary: xs)
+  case 0 thus ?case by (cases xs) auto
+next
+  case (Suc n) thus ?case by (cases xs) auto
+qed
+
+text \<open>Reverse of \<open>enabled_clause_body\<close>: an action whose translated positive-precondition atom
+  instances all hold in \<open>M\<close> and whose equality conditions are satisfied is enabled at \<open>M\<close>. The
+  precondition formula is rebuilt from its \<open>un_and\<close> literals (\<open>un_and_map_semantics_rev\<close>); the two
+  numeric side conditions are vacuous under \<open>nne\<close>.\<close>
+lemma clause_body_enabled:
+  assumes nne: "\<forall>a \<in> set (actions D). numeric_effects (ac_eff a) = []"
+    and sch_mem: "ac \<in> set (actions D)" and sch_name: "ac_name ac = n"
+    and pm: "action_params_match (ac_head ac) args"
+    and pos: "set (map (map_atom_fmla (ac_tsubst (cl_params (as_action_clause ac)) args))
+                 (cl_pred_pre (as_action_clause ac))) \<subseteq> fst M"
+    and sat: "satisfies_conds (cl_params (as_action_clause ac))
+                 (cl_cond_pre (as_action_clause ac)) args"
+  shows "plan_action_enabled (SimplePlanAction n args) M"
+proof -
+  obtain n' ps pre ad dl nl where sch_eq0:
+      "ac = SimpleActionSchema (ActionHead n' ps) (SimpleActionBody pre (Effect ad dl nl))"
+    by (metis ast_classical_action_schema_cases_unfold ast_effect.exhaust)
+  have nm: "n' = n" using sch_name sch_eq0 by simp
+  have ac_eq: "ac = SimpleActionSchema (ActionHead n ps) (SimpleActionBody pre (Effect ad dl nl))"
+    using sch_eq0 nm by simp
+  have cl_params: "cl_params (as_action_clause ac) = ps" using ac_eq by simp
+  have cl_pred: "cl_pred_pre (as_action_clause ac) = pos_lits_of pre" using ac_eq by simp
+  have cl_cond: "cl_cond_pre (as_action_clause ac) = cond_lits_of pre" using ac_eq by simp
+  let ?a' = "(the \<circ> res_inst) (SimplePlanAction n args)"
+  have res: "res_inst (SimplePlanAction n args)
+              = Some (GroundAction (map_atom_fmla (ac_tsubst ps args) pre)
+                                   (map_ast_effect (ac_tsubst ps args) (Effect ad dl nl)))"
+    using res_inst_cond[OF sch_mem[unfolded ac_eq]] .
+  have pre_eq: "precondition ?a' = map_atom_fmla (ac_tsubst ps args) pre" using res by simp
+  have eff_eq: "effect ?a' = map_ast_effect (ac_tsubst ps args) (Effect ad dl nl)"
+    using res by simp
+  have ne0: "numeric_effects (ac_eff ac) = []" using nne sch_mem by blast
+  have nl0: "nl = []" using ne0 ac_eq by simp
+  have numeff0: "numeric_effects (effect ?a') = []" unfolding eff_eq by (simp add: nl0)
+  have pos_conj: "is_pos_conj pre"
+  proof -
+    have "\<forall>a\<in>set (actions D). is_pos_conj (ac_pre a)"
+      using relaxed_prob by (auto simp: relaxed_prob_def relaxed_dom_def)
+    hence "is_pos_conj (ac_pre ac)" using sch_mem by simp
+    thus ?thesis using ac_eq by simp
+  qed
+  have val_pre: "valuation M \<Turnstile>\<^sub>m map_atom_fmla (ac_tsubst ps args) pre"
+  proof (rule un_and_map_semantics_rev, unfold un_and_map_atom_fmla, rule ballI)
+    fix g assume "g \<in> set (map (map_atom_fmla (ac_tsubst ps args)) (un_and pre))"
+    then obtain l where l: "l \<in> set (un_and pre)"
+      and g: "g = map_atom_fmla (ac_tsubst ps args) l" by auto
+    show "valuation M \<Turnstile>\<^sub>m g" unfolding g
+    proof (cases "is_predAtom l")
+      case True
+      hence l_pos: "l \<in> set (pos_lits_of pre)" using l by (simp add: pos_lits_of_def)
+      then obtain p xs where l_eq: "l = Atom (predAtm p xs)"
+        using True by (cases l rule: is_predAtom.cases) auto
+      have "map_atom_fmla (ac_tsubst ps args) l
+              \<in> set (map (map_atom_fmla (ac_tsubst ps args)) (cl_pred_pre (as_action_clause ac)))"
+        using l_pos cl_pred by auto
+      hence "map_atom_fmla (ac_tsubst ps args) l \<in> fst M" using pos cl_params by auto
+      thus "valuation M \<Turnstile>\<^sub>m map_atom_fmla (ac_tsubst ps args) l"
+        unfolding l_eq by (simp add: valuation_def)
+    next
+      case False
+      hence l_cond: "l \<in> set (cond_lits_of pre)" using l by (simp add: cond_lits_of_def)
+      have posl: "is_pos_lit l" using pos_conj l is_pos_conj_alt by blast
+      have "satisfies_cond ps args l"
+        using sat l_cond cl_cond cl_params by (simp add: list_all_iff)
+      hence "valuation ({}, Map.empty) \<Turnstile>\<^sub>m map_atom_fmla (ac_tsubst ps args) l" by simp
+      thus "valuation M \<Turnstile>\<^sub>m map_atom_fmla (ac_tsubst ps args) l"
+        using cond_lit_model_indep[OF posl False] by blast
+    qed
+  qed
+  have wf: "wf_classical_plan_action (SimplePlanAction n args)"
+    using wf_classical_plan_action_cond[OF sch_mem sch_name] pm by simp
+  show ?thesis
+    unfolding plan_action_enabled_def Let_def
+  proof (intro conjI)
+    show "wf_classical_plan_action (SimplePlanAction n args)" using wf .
+    show "numeric_effects_non_intrf ?a'"
+      by (rule numeric_effects_non_intrf_no_numeric_effects[OF numeff0])
+    show "set (ast_effect_enumerate_rhs_primitive_numeric_expressions (effect ?a')) \<subseteq> dom (snd M)"
+      using enumerate_rhs_pnes_no_numeric_effects[OF numeff0] by simp
+    show "valuation M \<Turnstile>\<^sub>m precondition ?a'" unfolding pre_eq using val_pre .
+  qed
+qed
+
+text \<open>Firing one action clause: if its translated argument tuple is well-typed, every
+  positive-precondition atom instance is achievable, and its equality conditions hold, then every
+  add-effect of the clause is achievable. The individually-achievable body facts are merged into a
+  common reachable state (\<open>achievables_reach_common\<close>), at which the action is enabled
+  (\<open>clause_body_enabled\<close>); firing it once produces the add-effect (\<open>execute_facts_eq\<close>,
+  \<open>res_inst_adds_eq_consequence\<close>).\<close>
+lemma fire_clause_achievable:
+  assumes nne: "\<forall>a \<in> set (actions D). numeric_effects (ac_eff a) = []"
+    and nd: "\<forall>a \<in> set (actions D). dels (ac_eff a) = []"
+    and cl_mem: "cl_ac \<in> set a_clauses"
+    and pm: "action_params_match (ActionHead (cl_name cl_ac) (cl_params cl_ac)) args"
+    and ach: "\<And>p xs. Atom (predAtm p xs) \<in> set (cl_pred_pre cl_ac)
+                \<Longrightarrow> achievable (p, map (ac_tsubst (cl_params cl_ac) args) xs)"
+    and sat: "satisfies_conds (cl_params cl_ac) (cl_cond_pre cl_ac) args"
+    and head: "Atom (predAtm p0 ts0) \<in> set (cl_pos cl_ac)"
+  shows "achievable (p0, map (ac_tsubst (cl_params cl_ac) args) ts0)"
+proof -
+  from cl_mem obtain sch where sch_mem: "sch \<in> set (actions D)"
+    and cl_eq: "cl_ac = as_action_clause sch" unfolding a_clauses_def by auto
+  obtain n ps pre ad dl nl where sch_eq:
+      "sch = SimpleActionSchema (ActionHead n ps) (SimpleActionBody pre (Effect ad dl nl))"
+    by (metis ast_classical_action_schema_cases_unfold ast_effect.exhaust)
+  have cl_eq': "cl_ac = AClause n ps (pos_lits_of pre) (cond_lits_of pre) ad"
+    using cl_eq sch_eq by simp
+  have cl_name: "cl_name cl_ac = n" and cl_params: "cl_params cl_ac = ps"
+    and cl_pos: "cl_pos cl_ac = ad" and cl_pred: "cl_pred_pre cl_ac = pos_lits_of pre"
+    using cl_eq' by simp_all
+  have sch_name: "ac_name sch = n" using sch_eq by simp
+  have head_eq: "ac_head sch = ActionHead n ps" using sch_eq by simp
+  have pm': "action_params_match (ac_head sch) args"
+    using pm cl_name cl_params head_eq by simp
+  have pred: "is_predAtom b" if "b \<in> set (cl_pred_pre cl_ac)" for b
+    using that cl_pred by (auto simp: pos_lits_of_def)
+  define fs where "fs = map (\<lambda>b. case b of Atom (predAtm p xs) \<Rightarrow> (p, map (ac_tsubst ps args) xs))
+                            (cl_pred_pre cl_ac)"
+  have achfs: "\<forall>f \<in> set fs. achievable f"
+  proof
+    fix f assume "f \<in> set fs"
+    then obtain b where b: "b \<in> set (cl_pred_pre cl_ac)"
+      and f_eq: "f = (case b of Atom (predAtm p xs) \<Rightarrow> (p, map (ac_tsubst ps args) xs))"
+      unfolding fs_def by (auto simp del: ac_tsubst_def)
+    from pred[OF b] obtain p xs where b_eq: "b = Atom (predAtm p xs)"
+      by (cases b rule: is_predAtom.cases) auto
+    have "achievable (p, map (ac_tsubst (cl_params cl_ac) args) xs)"
+      using ach b b_eq by auto
+    hence "achievable (p, map (ac_tsubst ps args) xs)" by (simp add: cl_params)
+    thus "achievable f" using f_eq b_eq by simp
+  qed
+  from achievables_reach_common[OF nne nd achfs] obtain \<pi>s Mstar
+    where vM: "valid_classical_plan_alt I \<pi>s Mstar"
+      and fsM: "\<forall>f \<in> set fs. Atom (uncurry predAtm f) \<in> fst Mstar" by blast
+  have pos: "set (map (map_atom_fmla (ac_tsubst ps args)) (cl_pred_pre cl_ac)) \<subseteq> fst Mstar"
+  proof
+    fix x assume "x \<in> set (map (map_atom_fmla (ac_tsubst ps args)) (cl_pred_pre cl_ac))"
+    then obtain b where b: "b \<in> set (cl_pred_pre cl_ac)"
+      and x: "x = map_atom_fmla (ac_tsubst ps args) b" by auto
+    from pred[OF b] obtain p xs where b_eq: "b = Atom (predAtm p xs)"
+      by (cases b rule: is_predAtom.cases) auto
+    have "(p, map (ac_tsubst ps args) xs) \<in> set fs" unfolding fs_def using b b_eq by force
+    hence "Atom (uncurry predAtm (p, map (ac_tsubst ps args) xs)) \<in> fst Mstar" using fsM by blast
+    moreover have "x = Atom (uncurry predAtm (p, map (ac_tsubst ps args) xs))"
+      using x b_eq by (simp add: uncurry_def)
+    ultimately show "x \<in> fst Mstar" by simp
+  qed
+  let ?pa = "SimplePlanAction n args"
+  have en: "plan_action_enabled ?pa Mstar"
+  proof (rule clause_body_enabled[OF nne sch_mem sch_name pm'])
+    show "set (map (map_atom_fmla (ac_tsubst (cl_params (as_action_clause sch)) args))
+                 (cl_pred_pre (as_action_clause sch))) \<subseteq> fst Mstar"
+      using pos by (simp add: cl_eq[symmetric] cl_params)
+    show "satisfies_conds (cl_params (as_action_clause sch))
+            (cl_cond_pre (as_action_clause sch)) args"
+      using sat by (simp add: cl_eq[symmetric])
+  qed
+  have fire: "valid_classical_plan_alt Mstar [?pa] (execute_plan_action ?pa Mstar)"
+    using en by (simp add: plan_action_enabled_def execute_plan_action_def)
+  have valid_full: "valid_classical_plan_alt I (\<pi>s @ [?pa]) (execute_plan_action ?pa Mstar)"
+    using valid_classical_plan_alt_append_intro[OF conjI[OF vM fire]] .
+  have adds_eq: "adds (effect ((the \<circ> res_inst) ?pa)) = consequence_of cl_ac args"
+    using res_inst_adds_eq_consequence[OF sch_mem[unfolded sch_eq]]
+    by (simp add: cl_eq sch_eq comp_def)
+  have conseq: "consequence_of cl_ac args = map (map_atom_fmla (ac_tsubst ps args)) (cl_pos cl_ac)"
+    using cl_eq' cl_pos by simp
+  have headmem: "Atom (predAtm p0 (map (ac_tsubst ps args) ts0))
+                   \<in> set (adds (effect ((the \<circ> res_inst) ?pa)))"
+  proof -
+    have "map_atom_fmla (ac_tsubst ps args) (Atom (predAtm p0 ts0)) \<in> set (consequence_of cl_ac args)"
+      unfolding conseq using head
+      by (auto simp del: ac_tsubst_def simp add: image_iff
+               intro!: bexI[where x="Atom (predAtm p0 ts0)"])
+    thus ?thesis unfolding adds_eq by simp
+  qed
+  have memN: "Atom (predAtm p0 (map (ac_tsubst ps args) ts0)) \<in> fst (execute_plan_action ?pa Mstar)"
+    using headmem execute_facts_eq[OF nd en] by auto
+  have "achievable (p0, map (ac_tsubst ps args) ts0)"
+    unfolding achievable_def
+    by (rule exI[of _ "\<pi>s @ [?pa]"], rule exI[of _ "execute_plan_action ?pa Mstar"])
+       (use valid_full memN in \<open>simp add: uncurry_def\<close>)
+  thus ?thesis using cl_params by simp
+qed
+
+text \<open>Every fact of \<^const>\<open>init'\<close> is achievable. A fact of \<^term>\<open>init P\<close> holds at the initial
+  state (\<open>init_achievable\<close>); a fact of \<^const>\<open>pseudo_init\<close> is the add-effect of a bodyless fact
+  clause fired at condition-satisfying object arguments --- the empty-body special case of
+  \<open>fire_clause_achievable\<close>.\<close>
+lemma init'_achievable:
+  assumes nne: "\<forall>a \<in> set (actions D). numeric_effects (ac_eff a) = []"
+    and nd: "\<forall>a \<in> set (actions D). dels (ac_eff a) = []"
+    and wf: "dl_bridge_wf P"
+    and mem: "Atom (predAtm p xs) \<in> set init'"
+  shows "achievable (p, xs)"
+proof -
+  from mem have "Atom (predAtm p xs) \<in> set pseudo_init \<or> Atom (predAtm p xs) \<in> set (init P)"
+    unfolding init'_def conc_unique_un by simp
+  thus ?thesis
+  proof
+    assume "Atom (predAtm p xs) \<in> set (init P)"
+    thus ?thesis by (rule init_achievable)
+  next
+    assume "Atom (predAtm p xs) \<in> set pseudo_init"
+    then obtain cl_ac where cl_fc: "cl_ac \<in> set fact_clauses"
+      and inafc: "Atom (predAtm p xs) \<in> set (all_fact_consqs cl_ac)"
+      unfolding pseudo_init_def by auto
+    then obtain args where args: "args \<in> set (all_fact_paramz cl_ac)"
+      and inconseq: "Atom (predAtm p xs) \<in> set (consequence_of cl_ac args)"
+      using inafc by auto
+    have cl_mem: "cl_ac \<in> set a_clauses" using cl_fc unfolding fact_clauses_def by simp
+    have cl_pred_empty: "cl_pred_pre cl_ac = []" using cl_fc unfolding fact_clauses_def by simp
+    from cl_mem obtain sch where sch_mem: "sch \<in> set (actions D)"
+      and cl_eq: "cl_ac = as_action_clause sch" unfolding a_clauses_def by auto
+    obtain n ps pre ad dl nl where sch_eq:
+        "sch = SimpleActionSchema (ActionHead n ps) (SimpleActionBody pre (Effect ad dl nl))"
+      by (metis ast_classical_action_schema_cases_unfold ast_effect.exhaust)
+    have cl_eq': "cl_ac = AClause n ps (pos_lits_of pre) (cond_lits_of pre) ad"
+      using cl_eq sch_eq by simp
+    have cl_name: "cl_name cl_ac = n" and cl_params: "cl_params cl_ac = ps"
+      and cl_cond: "cl_cond_pre cl_ac = cond_lits_of pre" and cl_pos: "cl_pos cl_ac = ad"
+      using cl_eq' by simp_all
+    have fp: "all_fact_paramz cl_ac
+                = all_combos (satisfies_conds ps (cond_lits_of pre)) (replicate (length ps) const_names)"
+      using cl_eq' by simp
+    have chosen: "chosen_from (replicate (length ps) const_names) args"
+      and satp: "satisfies_conds ps (cond_lits_of pre) args"
+      using args fp by (auto simp: set_all_combos)
+    from chosen_from_replicate_dest[OF chosen] have lenargs: "length args = length ps"
+      and inc: "\<forall>x \<in> set args. x \<in> set const_names" by auto
+    have pm: "action_params_match (ActionHead (cl_name cl_ac) (cl_params cl_ac)) args"
+    proof -
+      have "action_params_match (ac_head sch) args"
+      proof (rule params_match_from_const_args[OF sch_mem])
+        show "length args = length (ac_params sch)" using lenargs sch_eq by simp
+        show "\<And>x. x \<in> set args \<Longrightarrow> x \<in> set const_names" using inc by blast
+      qed
+      thus ?thesis using cl_name cl_params sch_eq by simp
+    qed
+    have sat: "satisfies_conds (cl_params cl_ac) (cl_cond_pre cl_ac) args"
+      using satp cl_params cl_cond by simp
+    have conseq: "consequence_of cl_ac args = map (map_atom_fmla (ac_tsubst ps args)) (cl_pos cl_ac)"
+      using cl_eq' cl_pos by simp
+    have "Atom (predAtm p xs) \<in> set (map (map_atom_fmla (ac_tsubst ps args)) (cl_pos cl_ac))"
+      using inconseq conseq by simp
+    then obtain f0 where f0: "f0 \<in> set (cl_pos cl_ac)"
+      and f0eq: "Atom (predAtm p xs) = map_atom_fmla (ac_tsubst ps args) f0" by auto
+    have "is_predAtom f0" using dl_bridge_wf_posD[OF wf cl_mem] f0 by blast
+    then obtain p0 ts0 where f0_pred: "f0 = Atom (predAtm p0 ts0)"
+      by (cases f0 rule: is_predAtom.cases) auto
+    have pxs: "p = p0 \<and> xs = map (ac_tsubst ps args) ts0" using f0eq f0_pred by simp
+    have head: "Atom (predAtm p0 ts0) \<in> set (cl_pos cl_ac)" using f0 f0_pred by simp
+    have ach: "achievable (p', map (ac_tsubst (cl_params cl_ac) args) xs')"
+      if "Atom (predAtm p' xs') \<in> set (cl_pred_pre cl_ac)" for p' xs'
+      using that cl_pred_empty by simp
+    have "achievable (p0, map (ac_tsubst (cl_params cl_ac) args) ts0)"
+      by (rule fire_clause_achievable[OF nne nd cl_mem pm ach sat head])
+    thus ?thesis using pxs cl_params by simp
+  qed
+qed
+
+text \<open>Inverting \<^const>\<open>dl_clauses_of_action_clause\<close>: a clause it produces has a predicate-atom add
+  effect as head and the translated precondition/condition body, and no literal failed to translate
+  (else the clause list would be empty). Dual to \<open>dl_clause_of_pos_mem\<close>.\<close>
+lemma dl_clause_of_action_clause_dest:
+  assumes "cl \<in> set (dl_clauses_of_action_clause cl_ac)"
+  obtains p ts where
+      "Atom (predAtm p ts) \<in> set (cl_pos cl_ac)"
+      "None \<notin> set (map dl_cond_rh (cl_cond_pre cl_ac))"
+      "None \<notin> set (map dl_pos_rh (cl_pred_pre cl_ac))"
+      "cl = Cls p (map dl_id_of_term ts) (dl_clause_body cl_ac)"
+proof -
+  let ?conds = "map dl_cond_rh (cl_cond_pre cl_ac)"
+  let ?pres = "map dl_pos_rh (cl_pred_pre cl_ac)"
+  let ?body = "dl_clause_body cl_ac"
+  have nN1: "None \<notin> set ?conds" and nN2: "None \<notin> set ?pres"
+  proof -
+    have "\<not> (None \<in> set ?conds \<or> None \<in> set ?pres)"
+    proof
+      assume "None \<in> set ?conds \<or> None \<in> set ?pres"
+      hence "dl_clauses_of_action_clause cl_ac = []"
+        unfolding dl_clauses_of_action_clause_def Let_def by auto
+      thus False using assms by simp
+    qed
+    thus "None \<notin> set ?conds" "None \<notin> set ?pres" by auto
+  qed
+  from assms nN1 nN2 obtain f where f: "f \<in> set (cl_pos cl_ac)"
+    and fc: "(case f of Atom (predAtm p ts) \<Rightarrow> Some (Cls p (map dl_id_of_term ts) ?body) | _ \<Rightarrow> None)
+               = Some cl"
+    unfolding dl_clauses_of_action_clause_def Let_def
+    by (auto simp add: set_map_filter' simp del: map_map split: if_split_asm)
+  from fc obtain p ts where "f = Atom (predAtm p ts)"
+    and "cl = Cls p (map dl_id_of_term ts) ?body"
+    by (auto split: formula.splits atom.splits)
+  thus ?thesis using f nN1 nN2 that by blast
+qed
+
+text \<open>Reverse of \<open>dl_cond_rh_eval_guard\<close>: a translated condition is satisfied (in the empty model)
+  whenever it is a drop-marker (\<open>Some None\<close>) or its equality guard holds under the
+  argument substitution.\<close>
+lemma dl_cond_rh_satisfies:
+  assumes nN: "dl_cond_rh cnd \<noteq> None"
+    and gd: "\<And>g. dl_cond_rh cnd = Some (Some g)
+               \<Longrightarrow> eval_guard (\<lambda>v. ac_tsubst ps args (term.VAR v)) g"
+  shows "satisfies_cond ps args cnd"
+  using assms
+  by (cases cnd rule: dl_cond_rh.cases)
+     (auto simp del: ac_tsubst_def simp add: valuation_def subst_id_dl_id_term)
+
+text \<open>Tightness / \<open>\<supseteq>\<close>: every fact of the minimal model is PDDL-achievable. Rule induction on
+  \<^const>\<open>datalog_prog.derivable\<close>. A derivation step fires a clause of \<^const>\<open>dl_rules\<close>: a
+  translated action clause (fire that action via \<open>fire_clause_achievable\<close>; its body-atom instances
+  are achievable by the IH, its equality guards give the conditions, and the argument tuple is
+  reconstructed from the generic substitution \<open>\<sigma>\<close>) or a bodyless fact clause from
+  \<^const>\<open>init'\<close> (\<open>init'_achievable\<close>). Needs the delete-relaxation / numeric-freeness hypotheses
+  \<open>nne\<close> / \<open>nd\<close> that \<open>fire_clause_achievable\<close> and \<open>init'_achievable\<close> carry.\<close>
+lemma dl_derivable_imp_achievable:
+  assumes nne: "\<forall>a \<in> set (actions D). numeric_effects (ac_eff a) = []"
+    and nd: "\<forall>a \<in> set (actions D). dels (ac_eff a) = []"
+    and wf: "dl_bridge_wf P"
+    and der: "dl_prog.derivable f"
+  shows "achievable f"
+proof -
+  note ind = dl_prog.derivable.induct[consumes 1, case_names step]
+  show ?thesis using der
+  proof (induction rule: ind)
+    case (step cl \<sigma>)
+    from step.hyps(1) consider
+        (act) cl_ac where "cl_ac \<in> set a_clauses" "cl \<in> set (dl_clauses_of_action_clause cl_ac)"
+      | (fct) "cl \<in> set (List.map_filter dl_fact_clause init')"
+      unfolding dl_rules_def by auto
+    thus ?case
+    proof cases
+      case (act cl_ac)
+      from dl_clause_of_action_clause_dest[OF act(2)] obtain p0 ts0 where
+          head: "Atom (predAtm p0 ts0) \<in> set (cl_pos cl_ac)"
+          and nc: "None \<notin> set (map dl_cond_rh (cl_cond_pre cl_ac))"
+          and np: "None \<notin> set (map dl_pos_rh (cl_pred_pre cl_ac))"
+          and cl_eq: "cl = Cls p0 (map dl_id_of_term ts0) (dl_clause_body cl_ac)" .
+      from act(1) obtain sch where sch_mem: "sch \<in> set (actions D)"
+        and cl_eq2: "cl_ac = as_action_clause sch" unfolding a_clauses_def by auto
+      obtain nm ps pre ad dl' nl where sch_eq:
+          "sch = SimpleActionSchema (ActionHead nm ps) (SimpleActionBody pre (Effect ad dl' nl))"
+        by (metis ast_classical_action_schema_cases_unfold ast_effect.exhaust)
+      have cl_params: "cl_params cl_ac = ps" and cl_name: "cl_name cl_ac = nm"
+        using cl_eq2 sch_eq by simp_all
+      have "wf_classical_action_schema sch" using wf_D(3) sch_mem by blast
+      hence "distinct (map fst (ac_params sch))" using wf_classical_action_schema_alt by blast
+      hence dist: "distinct (map fst ps)" using sch_eq by simp
+      have cn_ne: "const_names \<noteq> []" using dl_bridge_wf_const_namesD[OF wf] .
+      define c0 where "c0 = hd const_names"
+      have c0_mem: "c0 \<in> set const_names" unfolding c0_def by (rule hd_in_set[OF cn_ne])
+      define args where
+        "args = map (\<lambda>vp. if fst vp \<in> set (cls_vars cl) then \<sigma> (fst vp) else c0) ps"
+      have lenargs: "length args = length ps" unfolding args_def by simp
+      have varsub: "set (cls_vars cl) \<subseteq> set (map fst ps)"
+        using dl_bridge_wf_varsD[OF wf act(1) act(2)] cl_params by simp
+      have agree: "ac_tsubst ps args (term.VAR x) = \<sigma> x" if x: "x \<in> set (cls_vars cl)" for x
+      proof -
+        from x varsub have "x \<in> set (map fst ps)" by auto
+        then obtain i where i: "i < length ps" and xi: "map fst ps ! i = x"
+          by (auto simp: in_set_conv_nth)
+        have psi: "ps ! i = (x, snd (ps ! i))" using xi i by (cases "ps ! i") auto
+        have fstx: "fst (ps ! i) = x" using xi i by simp
+        have ai: "args ! i = \<sigma> x" unfolding args_def using i fstx x by simp
+        have il: "i < length args" using i lenargs by simp
+        show ?thesis by (rule ac_tsubst_intro[OF dist psi ai i il])
+      qed
+      have subst_eq: "subst_id \<sigma> (dl_id_of_term t) = ac_tsubst ps args t"
+        if "\<And>v. t = term.VAR v \<Longrightarrow> v \<in> set (cls_vars cl)" for t
+      proof (cases t)
+        case (VAR v)
+        hence hv: "v \<in> set (cls_vars cl)" using that by simp
+        show ?thesis unfolding VAR using agree[OF hv] by (simp del: ac_tsubst_def)
+      next
+        case (CONST c)
+        thus ?thesis by simp
+      qed
+      have args_const: "a \<in> set const_names" if "a \<in> set args" for a
+      proof -
+        from that obtain vp where vp: "vp \<in> set ps"
+          and a_eq: "a = (if fst vp \<in> set (cls_vars cl) then \<sigma> (fst vp) else c0)"
+          unfolding args_def by auto
+        show ?thesis
+        proof (cases "fst vp \<in> set (cls_vars cl)")
+          case True
+          hence "a = \<sigma> (fst vp)" using a_eq by simp
+          thus ?thesis using step.hyps(2) True by auto
+        next
+          case False
+          thus ?thesis using a_eq c0_mem by simp
+        qed
+      qed
+      have head_vars: "v \<in> set (cls_vars cl)" if "t \<in> set ts0" "t = term.VAR v" for t v
+      proof -
+        have "dl_id_of_term t \<in> set (snd (the_lh cl))" using that(1) by (simp add: cl_eq)
+        moreover have "v \<in> set (id_vars_list (dl_id_of_term t))" using that(2) by simp
+        ultimately show ?thesis by (rule cls_vars_head_vars)
+      qed
+      have lh_eq: "subst_atom \<sigma> (the_lh cl) = (p0, map (ac_tsubst ps args) ts0)"
+      proof -
+        have "map (subst_id \<sigma>) (map dl_id_of_term ts0) = map (ac_tsubst ps args) ts0"
+        proof (subst map_map, rule map_cong[OF refl])
+          fix t assume "t \<in> set ts0"
+          thus "(subst_id \<sigma> \<circ> dl_id_of_term) t = ac_tsubst ps args t"
+            using subst_eq[OF head_vars[OF \<open>t \<in> set ts0\<close>]] by (simp del: ac_tsubst_def)
+        qed
+        thus ?thesis unfolding cl_eq subst_atom_def by (simp del: ac_tsubst_def)
+      qed
+      have pmh: "action_params_match (ac_head sch) args"
+      proof (rule params_match_from_const_args[OF sch_mem])
+        show "length args = length (ac_params sch)" using lenargs sch_eq by simp
+        show "\<And>a. a \<in> set args \<Longrightarrow> a \<in> set const_names" using args_const by blast
+      qed
+      have pm: "action_params_match (ActionHead (cl_name cl_ac) (cl_params cl_ac)) args"
+        using pmh sch_eq cl_name cl_params by simp
+      have ach: "achievable (p', map (ac_tsubst (cl_params cl_ac) args) xs')"
+        if pre': "Atom (predAtm p' xs') \<in> set (cl_pred_pre cl_ac)" for p' xs'
+      proof -
+        have rh_mem: "PosLit p' (map dl_id_of_term xs') \<in> set (the_rhs cl)"
+        proof -
+          have "the (dl_pos_rh (Atom (predAtm p' xs')))
+                  \<in> set (map the (map dl_pos_rh (cl_pred_pre cl_ac)))" using pre' by force
+          thus ?thesis using cl_eq by (simp add: dl_clause_body_def)
+        qed
+        hence body_mem: "(p', map dl_id_of_term xs') \<in> set (cls_body_atoms cl)"
+          by (simp add: cls_body_atoms_iff)
+        have body_vars: "v \<in> set (cls_vars cl)" if tv: "t \<in> set xs'" "t = term.VAR v" for t v
+        proof -
+          have "term.VAR v \<in> set xs'" using tv by simp
+          hence "v \<in> set (rh_vars_list (PosLit p' (map dl_id_of_term xs')))" by force
+          thus ?thesis using cls_vars_rhs_vars[OF rh_mem] by blast
+        qed
+        have "map (subst_id \<sigma>) (map dl_id_of_term xs') = map (ac_tsubst ps args) xs'"
+        proof (subst map_map, rule map_cong[OF refl])
+          fix t assume "t \<in> set xs'"
+          thus "(subst_id \<sigma> \<circ> dl_id_of_term) t = ac_tsubst ps args t"
+            using subst_eq[OF body_vars[OF \<open>t \<in> set xs'\<close>]] by (simp del: ac_tsubst_def)
+        qed
+        hence "subst_atom \<sigma> (p', map dl_id_of_term xs') = (p', map (ac_tsubst ps args) xs')"
+          unfolding subst_atom_def by simp
+        moreover have "achievable (subst_atom \<sigma> (p', map dl_id_of_term xs'))"
+          using step.IH body_mem by blast
+        ultimately show ?thesis using cl_params by simp
+      qed
+      have sat: "satisfies_conds (cl_params cl_ac) (cl_cond_pre cl_ac) args"
+        unfolding cl_params list_all_iff
+      proof
+        fix cnd assume cnd: "cnd \<in> set (cl_cond_pre cl_ac)"
+        show "satisfies_cond ps args cnd"
+        proof (rule dl_cond_rh_satisfies)
+          show "dl_cond_rh cnd \<noteq> None"
+          proof
+            assume "dl_cond_rh cnd = None"
+            hence "None \<in> set (map dl_cond_rh (cl_cond_pre cl_ac))" using cnd by force
+            thus False using nc by simp
+          qed
+        next
+          fix g assume g: "dl_cond_rh cnd = Some (Some g)"
+          have "Some g \<in> set (map the (map dl_cond_rh (cl_cond_pre cl_ac)))"
+            using cnd g by force
+          hence "g \<in> set (List.map_filter id (map the (map dl_cond_rh (cl_cond_pre cl_ac))))"
+            by (auto simp: set_map_filter')
+          hence g_rhs: "g \<in> set (the_rhs cl)" using cl_eq by (simp add: dl_clause_body_def)
+          have "is_dl_guard g" using g by (cases cnd rule: dl_cond_rh.cases) auto
+          hence g_grd: "g \<in> set (cls_guards cl)" using g_rhs by (simp add: cls_guards_def)
+          have ev: "eval_guard \<sigma> g" using step.hyps(3) g_grd by blast
+          have "\<forall>x \<in> set (rh_vars_list g). \<sigma> x = (\<lambda>v. ac_tsubst ps args (term.VAR v)) x"
+          proof
+            fix x assume xr: "x \<in> set (rh_vars_list g)"
+            have xcv: "x \<in> set (cls_vars cl)" using cls_vars_rhs_vars[OF g_rhs] xr by blast
+            show "\<sigma> x = (\<lambda>v. ac_tsubst ps args (term.VAR v)) x"
+              using agree[OF xcv] by (simp del: ac_tsubst_def)
+          qed
+          hence "eval_guard \<sigma> g = eval_guard (\<lambda>v. ac_tsubst ps args (term.VAR v)) g"
+            by (rule eval_guard_agree)
+          thus "eval_guard (\<lambda>v. ac_tsubst ps args (term.VAR v)) g" using ev by simp
+        qed
+      qed
+      have "achievable (p0, map (ac_tsubst (cl_params cl_ac) args) ts0)"
+        by (rule fire_clause_achievable[OF nne nd act(1) pm ach sat head])
+      thus "achievable (subst_atom \<sigma> (the_lh cl))" using lh_eq cl_params by simp
+    next
+      case fct
+      then obtain f0 where f0: "f0 \<in> set init'" and dfc: "dl_fact_clause f0 = Some cl"
+        unfolding set_map_filter' by auto
+      from dfc obtain pp xs where f0_eq: "f0 = Atom (predAtm pp xs)"
+        and cl_eq: "cl = Cls pp (map id.Cst xs) []"
+        by (cases f0 rule: dl_fact_clause.cases) auto
+      have "Atom (predAtm pp xs) \<in> set init'" using f0 f0_eq by simp
+      hence "achievable (pp, xs)" by (rule init'_achievable[OF nne nd wf])
+      moreover have "subst_atom \<sigma> (the_lh cl) = (pp, xs)"
+        unfolding cl_eq subst_atom_def by (simp add: comp_def)
+      ultimately show "achievable (subst_atom \<sigma> (the_lh cl))" by simp
+    qed
+  qed
+qed
+
+text \<open>PDDL reachability is exactly the minimal datalog model: \<open>\<subseteq>\<close> (soundness) is unconditional,
+  \<open>\<supseteq>\<close> (tightness) needs the delete-relaxation / numeric-freeness hypotheses \<open>nne\<close> / \<open>nd\<close>.\<close>
 theorem achievable_eq_minimal_model:
-  assumes "dl_bridge_wf P"
-  shows "{f. achievable f} = {f. datalog_prog.derivable (set const_names) (set (dl_rules P)) f}"
-  using achievable_imp_dl_derivable[OF assms] dl_derivable_imp_achievable[OF assms] by blast
+  assumes nne: "\<forall>a \<in> set (actions D). numeric_effects (ac_eff a) = []"
+    and nd: "\<forall>a \<in> set (actions D). dels (ac_eff a) = []"
+    and wf: "dl_bridge_wf P"
+  shows "{f. achievable f} = {f. dl_prog.derivable f}"
+  using achievable_imp_dl_derivable[OF wf] dl_derivable_imp_achievable[OF nne nd wf] by blast
 
 subsection \<open>Relating an admissible certificate to PDDL reachability\<close>
 
@@ -572,13 +1656,15 @@ text \<open>The capstone: any list \<open>M\<close> that the \<^emph>\<open>gene
   PDDL-achievable facts of the relaxed problem. An accepted \<^const>\<open>dl_admissible\<close> certificate
   thus yields the reachable-fact set by theorem, with no PDDL-specific check.\<close>
 theorem certified_facts_eq_achievable:
-  assumes wf: "dl_bridge_wf P"
+  assumes nne: "\<forall>a \<in> set (actions D). numeric_effects (ac_eff a) = []"
+    and nd: "\<forall>a \<in> set (actions D). dels (ac_eff a) = []"
+    and wf: "dl_bridge_wf P"
     and cert: "dl_certified_model (set (dl_rules P)) (set const_names) M dc"
   shows "set M = {f. achievable f}"
 proof -
-  have "{f. achievable f} = {f. datalog_prog.derivable (set const_names) (set (dl_rules P)) f}"
-    by (rule achievable_eq_minimal_model[OF wf])
-  with dl_certified_model_correct[OF cert] show ?thesis by simp
+  have "{f. achievable f} = {f. dl_prog.derivable f}"
+    by (rule achievable_eq_minimal_model[OF nne nd wf])
+  thus ?thesis using dl_certified_model_correct[OF cert] by simp
 qed
 
 text \<open>The facts requirement, discharged by a certified minimal model: the facts of any certified
@@ -586,13 +1672,54 @@ text \<open>The facts requirement, discharged by a certified minimal model: the 
   established without any PDDL-specific closure check.\<close>
 theorem minimal_model_facts_requirement:
   assumes wf: "dl_bridge_wf P"
-    and model: "set M = {f. datalog_prog.derivable (set const_names) (set (dl_rules P)) f}"
+    and model: "set M = {f. dl_prog.derivable f}"
   shows "fact_to_facty ` {f. achievable f} \<subseteq> fact_to_facty ` set M"
 proof -
   have "{f. achievable f} \<subseteq> set M"
     using achievable_imp_dl_derivable[OF wf] model by blast
   thus ?thesis by (rule image_mono)
 qed
+
+end
+
+
+subsection \<open>The grounding-input locale: numeric-free, delete-relaxed, well-translated\<close>
+
+text \<open>The pipeline grounds \<open>relax_prob (P\<^sub>T P)\<close> --- a \<^emph>\<open>numeric-free\<close> (def-translated) and
+  \<^emph>\<open>delete-relaxed\<close> problem whose datalog translation is well-formed. This locale bundles exactly
+  those three facts on top of \<^locale>\<open>pddl_datalog\<close>, so the reachability capstones hold \<^emph>\<open>without\<close>
+  explicit hypotheses. (Deriving \<open>nne\<close> from \<open>num_free_prob\<close> and proving \<open>dl_bridge_wf\<close> from
+  numeric-freeness + relaxation + well-formedness + a non-empty object universe specialises these
+  assumptions further; that needs \<open>Tree_Decomp_Grounding_Common.Numeric_Free\<close> on this
+  theory's import path.)\<close>
+locale num_free_relaxed_problem = pddl_datalog + numeric_free_problem +
+  assumes bridge: "dl_bridge_wf P"
+begin
+
+text \<open>No numeric effects --- derived from numeric-freeness (a numeric-free effect has an empty
+  numeric-effect list).\<close>
+lemma nne: "\<forall>a \<in> set (actions D). numeric_effects (ac_eff a) = []"
+proof
+  fix a assume "a \<in> set (actions D)"
+  hence "num_free_ac a" using num_free_dom unfolding num_free_dom_def by blast
+  thus "numeric_effects (ac_eff a) = []" unfolding num_free_ac_def by (cases "ac_eff a") auto
+qed
+
+text \<open>Empty deletes --- now part of \<^const>\<open>relaxed_prob\<close> (delete relaxation folded into
+  \<^locale>\<open>relaxed_problem\<close>).\<close>
+lemma nd: "\<forall>a \<in> set (actions D). dels (ac_eff a) = []"
+  using relaxed_prob by (auto simp: relaxed_prob_def relaxed_dom_def)
+
+text \<open>PDDL reachability is exactly the minimal datalog model --- unconditionally in this locale.\<close>
+theorem reachable_eq_minimal_model:
+  "{f. achievable f} = {f. dl_prog.derivable f}"
+  by (rule achievable_eq_minimal_model[OF nne nd bridge])
+
+text \<open>An accepted generic certificate's facts are exactly the reachable facts.\<close>
+theorem certified_facts_eq_reachable:
+  assumes "dl_certified_model (set (dl_rules P)) (set const_names) M dc"
+  shows "set M = {f. achievable f}"
+  by (rule certified_facts_eq_achievable[OF nne nd bridge assms])
 
 end
 
